Common/Util.lean
@@ -1,8 +1,15 @@
 
+import Common.Mathlib
 
 def contra {A B} : (A -> B) -> Not B -> Not A := by
   intros h1 h2 h3
   exact (h2 (h1 h3))
+
+lemma demorgan : ¬ (A ∨ B) -> ¬ A ∧ ¬ B := by {
+  intro h; apply And.intro _ _
+  intro h2; apply h (Or.inl h2)
+  intro h2; apply h (Or.inr h2)
+}
 
 def ne_sym : x ≠ y -> y ≠ x := sorry 
 
@@ -11,3 +18,7 @@ def append_eq {a c : List α} {b d : α} : a ++ [b] = c ++ [d] -> a = c ∧ b = 
 def pair_eq : (a, b) = (c, d) -> a = c ∧ b = d := sorry
 
 def nat_add_le {a b c : Nat} : a + b ≤ c -> a ≤ c ∧ b ≤ c := sorry  
+
+def fin_cast {i u : Nat} : (h : i < i + 1) -> Fin.mk i h = ↑i := sorry
+
+def fin_cast2 {n : Nat} {i : Fin (n + 1)} : i = ↑i.val := sorry
