Cedille/Lemma/Basic.lean
@@ -17,10 +17,6 @@ namespace Cedille
     unfold HasHOpen.hopn; unfold Syntax.instHasHOpenSyntax; simp
     unfold Syntax.opn_head; simp; unfold bound; simp; unfold free; simp
   }
-  
-  @[simp] def open_free : {_|-> y}(@free (n + 1) x) = free x := by {
-    unfold free; simp
-  }
 
   @[simp] lemma fv_id_empty : @fv n (lam mf kindu (bound 0)) = [] := by {
     unfold lam; unfold fv; unfold Syntax.fv;
@@ -28,29 +24,27 @@ namespace Cedille
     unfold bound; simp;
   }
 
-  @[simp] lemma mode_pi_domain_mf : Mode.pi_domain mf K = typeu := by congr
-  @[simp] lemma mode_pi_domain_m0 : Mode.pi_domain m0 K = const K := by congr
-  @[simp] lemma mode_pi_domain_mt : Mode.pi_domain mt K = const K := by congr
+  @[simp] lemma mode_pi_domain_mf : Mode.pi_domain mf K = @typeu n := by congr
+  @[simp] lemma mode_pi_domain_m0 : Mode.pi_domain m0 K = @const n K := by congr
+  @[simp] lemma mode_pi_domain_mt : Mode.pi_domain mt K = @const n K := by congr
 
-  lemma conv_mode_pi_domain : A =β= Mode.pi_domain m K -> A -β>* Mode.pi_domain m K := by {
-    intros h; cases h; case _ t1 t2 s1 s2 e =>
-    
-  }
+  @[simp] lemma mode_pi_codomain_mf : Mode.pi_codomain mf = @typeu n := by congr
+  @[simp] lemma mode_pi_codomain_m0 : Mode.pi_codomain m0 = @typeu n := by congr
+  @[simp] lemma mode_pi_codomain_mt : Mode.pi_codomain mt = @kindu n := by congr
 
-  @[simp] lemma mode_pi_codomain_mf : Mode.pi_codomain mf = typeu := by congr
-  @[simp] lemma mode_pi_codomain_m0 : Mode.pi_codomain m0 = typeu := by congr
-  @[simp] lemma mode_pi_codomain_mt : Mode.pi_codomain mt = kindu := by congr
+  @[simp] lemma mode_lam_domain_mf : Mode.lam_domain mf = @typeu n := by congr
+  @[simp] lemma mode_lam_domain_m0 : Mode.lam_domain m0 = @typeu n := by congr
+  @[simp] lemma mode_lam_domain_mt : Mode.lam_domain mt = @kindu n := by congr
 
-  @[simp] lemma mode_lam_domain_mf : Mode.lam_domain mf = typeu := by congr
-  @[simp] lemma mode_lam_domain_m0 : Mode.lam_domain m0 = typeu := by congr
-  @[simp] lemma mode_lam_domain_mt : Mode.lam_domain mt = kindu := by congr
+  lemma subset_mem {x : Name} {A B : FvSet!} : A ⊆ B -> x ∈ A -> x ∈ B := sorry
+  @[simp] lemma fv_subst : fv ([_:= t1]t2) = fv t1 ++ fv t2 := sorry
+  @[simp] lemma fv_open : fv ({_|-> x}t) = [x] ++ fv t := sorry
 
-  @[simp] lemma open_lambda : {_|-> x}lam m t1 t2 = lam m ({_|-> x}t1) ({_|-> x}t2) := by {
-    unfold lam; simp
-  }
+  lemma subset_left {A B C : FvSet!} : A ⊆ B -> A ⊆ B ++ C := sorry
+  lemma subset_right {A B C : FvSet!} : A ⊆ C -> A ⊆ B ++ C := sorry
+  lemma subset_cons {A B : FvSet!} : x ∉ A -> A ⊆ x :: B -> A ⊆ B := sorry
+  lemma subset_trans {A B C : FvSet!} : A ⊆ B -> B ⊆ C -> A ⊆ C := sorry 
 
-  @[simp] lemma open_pi : {_|-> x}pi m t1 t2 = pi m ({_|-> x}t1) ({_|-> x}t2) := by {
-    unfold pi; simp
-  }
+  lemma not_mem_subset_not_mem {A B : FvSet!} : x ∉ A -> B ⊆ A -> x ∉ B := sorry
 
 end Cedille
