Cedille/Lemma/Erasure.lean
@@ -2,6 +2,7 @@
 import Common
 import Cedille.Def
 import Cedille.Lemma.Refold
+import Cedille.Lemma.Inversion
 
 namespace Cedille
 
@@ -39,10 +40,11 @@ namespace Cedille
     rfl
   }
 
-  @[simp] lemma erase_app_m0 : erase (t1 @0 t2) = erase t1 := by generalize erase t1 = t; rfl
+  @[simp] lemma erase_app_m0 : erase (t1 @0 t2) = erase t1
+    := by rfl
   @[simp] lemma erase_app_m0_unfolded
     : erase (Syntax.ctor (Constructor.app m0) t1 t2 t3) = erase t1
-  := by generalize erase t1 = t; rfl
+  := by rfl
 
   @[simp] lemma erase_app_mf : erase (t1 @ω t2) = (erase t1) @ω (erase t2) := by congr
   @[simp] lemma erase_app_mf_unfolded
@@ -60,22 +62,24 @@ namespace Cedille
     unfold erase; simp only; subst h; rfl
   }
 
-  @[simp] lemma erase_pair : erase (pair t1 t2 t3) = erase t1 := by generalize erase t1 = t; rfl
+  @[simp] lemma erase_pair : erase (pair t1 t2 t3) = erase t1
+    := rfl
   @[simp] lemma erase_pair_unfolded
-    : erase (Syntax.ctor Constructor.pair t1 t2 t3) = erase t1
-  := by generalize erase t1 = t; rfl
+    : erase (Syntax.ctor Constructor.pair t1 t2 t3) =erase t1
+  := rfl
 
-  @[simp] lemma erase_fst : erase (fst t) = erase t := by generalize erase t = s; rfl
+  @[simp] lemma erase_fst : erase (fst t) = erase t := by generalize t = s; rfl
   @[simp] lemma erase_fst_unfolded
-    : erase (Syntax.ctor Constructor.fst t1 t2 t3) = erase t1
-  := by generalize erase t1 = t; rfl
+    : erase (Syntax.ctor Constructor.fst t1 t2 t3) =erase t1
+  := rfl
 
-  @[simp] lemma erase_snd : erase (snd t) = erase t := by generalize erase t = s; rfl
+  @[simp] lemma erase_snd : erase (snd t) = erase t := by generalize t = s; rfl
   @[simp] lemma erase_snd_unfolded
-    : erase (Syntax.ctor Constructor.snd t1 t2 t3) = erase t1
-  := by generalize erase t1 = t; rfl
+    : erase (Syntax.ctor Constructor.snd t1 t2 t3) =erase t1
+  := rfl
 
-  @[simp] lemma erase_eq : erase (eq t1 t2 t3) = eq (erase t1) (erase t2) (erase t3) := by congr
+  @[simp] lemma erase_eq : erase (eq t1 t2 t3) = eq (erase t1) (erase t2) (erase t3)
+    := by congr
   @[simp] lemma erase_eq_unfolded
     : erase (Syntax.ctor Constructor.eq t1 t2 t3) = eq (erase t1) (erase t2) (erase t3)
   := by {
@@ -93,22 +97,17 @@ namespace Cedille
     : erase (Syntax.ctor Constructor.eqind t1 t2 t3) = lam mf kindu (bound 0)
   := by congr
 
-  @[simp] lemma erase_promote : erase (promote t) = erase t := by generalize erase t = t; rfl
+  @[simp] lemma erase_promote : erase (promote t) = erase t := by rfl
   @[simp] lemma erase_promote_unfolded
     : erase (Syntax.ctor Constructor.promote t1 t2 t3) = erase t1
-  := by generalize erase t1 = t; rfl
+  := rfl
 
-  @[simp] lemma erase_deltatop : erase (deltatop t) = erase t := by generalize erase t = s; rfl
-  @[simp] lemma erase_deltatop_unfolded
-    : erase (Syntax.ctor Constructor.deltatop t1 t2 t3) = erase t1
-  := by generalize erase t1 = t; rfl
+  @[simp] lemma erase_delta : erase (delta t) = erase t := by rfl
+  @[simp] lemma erase_delta_unfolded
+    : erase (Syntax.ctor Constructor.delta t1 t2 t3) = erase t1
+  := by rfl
 
-  @[simp] lemma erase_deltabot : erase (deltabot t) = erase t := by generalize erase t = s; rfl
-  @[simp] lemma erase_deltabot_unfolded
-    : erase (Syntax.ctor Constructor.deltabot t1 t2 t3) = erase t1
-  := by generalize erase t1 = t; rfl
-
-  @[simp] lemma erase_phi : erase (phi t1 t2 t3) = erase t1 := by generalize erase t1 = t; rfl
+  @[simp] lemma erase_phi : erase (phi t1 t2 t3) = erase t1 := by rfl
 
   @[simp] lemma erase_idem {m} {t : Term m} : erase (erase t) = erase t := @Nat.rec
     (λ n => {m : Nat} -> (t : Term m) -> size t ≤ n -> erase (erase t) = erase t)
@@ -124,18 +123,9 @@ namespace Cedille
         have h := nat_add_le h
         casesm* _ ∧ _
         case _ h1 h2 =>
-        have lem1 := ih t1 h1
-        have lem2 := ih t2 h2
         cases k <;> simp [*]
         case lam k =>
         cases k <;> simp [*]
-        case erased =>
-        have lem := @Syntax.size_opn_head _ _ _ _ (Name.fresh (fv t2)) t2
-        rewrite [Cedille.size_size, Cedille.size_size] at lem
-        rewrite [<-lem] at h2
-        have lem := ih _ h2
-        rewrite [lem]
-        rfl
       }
       case ctor k t1 t2 t3 => {
         have h := Nat.le_of_succ_le_succ h
@@ -155,27 +145,40 @@ namespace Cedille
     t
     (by simp)
 
-  @[simp] lemma erase_subst : erase ([_:= a]f) = [_:= erase a](erase f) := sorry
+  lemma erase_rename : erase t1 = erase t2 -> erase ({_|-> x}{_<-| y}t1) = erase ({_|-> x}{_<-| y}t2)
+  := by sorry
 
-  lemma erase_close_open : erase t = {_|-> x}s -> erase ({_<-| x}t) = s := sorry
+  lemma erase_free_rename :
+    ((x : Name) -> x ∉ fv t -> x ∉ (fv ∘ erase) ({_|-> x}t)) ->
+    (x y : Name) -> x ∉ fv t -> y ∉ fv t -> erase ({_|-> x}t) = erase ({_|-> y}t)
+  := by {
+    intro h x y xnin ynin
+    have hx := h x xnin
+    have hy := h y ynin
+    sorry
+  }
 
-  lemma erase_forces_lam_mt : erase f = lam mt t1 t2 ->
-    ∃ t1' t2', erase t1' = t1 ∧ erase t2' = t2 ∧ f = lam mt t1' t2'
-  := sorry
+  -- @[simp] lemma erase_subst : erase ([_:= a]f) = [_:= erase a](erase f) := sorry
 
-  lemma erase_forces_lam_mf : erase f = lam mf t1 t2 ->
-    ∃ t1' t2', erase t1' = t1 ∧ erase t2' = t2 ∧ f = lam mf t1' t2'
-  := sorry
+  -- lemma erase_close_open : erase t = {_|-> x}s -> erase ({_<-| x}t) = s := sorry
 
-  lemma erase_no_eqind : erase f ≠ J @τ t1 @τ t2 @0 t3 @0 t4 @ω t5 := sorry
+  -- lemma erase_forces_lam_mt : erase f = lam mt t1 t2 ->
+  --   ∃ t1' t2', erase t1' = t1 ∧ erase t2' = t2 ∧ f = lam mt t1' t2'
+  -- := sorry
 
-  lemma erase_free_invariant :
-    x ∉ (fv ∘ erase) ({_|-> x}t) ->
-    (y : Name) -> y ∉ fv t ->
-    erase ({_|-> x}t) = erase ({_|-> y}t)
-  := sorry
+  -- lemma erase_forces_lam_mf : erase f = lam mf t1 t2 ->
+  --   ∃ t1' t2', erase t1' = t1 ∧ erase t2' = t2 ∧ f = lam mf t1' t2'
+  -- := sorry
 
-  lemma erase_ctt_eq : erase t = erase ctt -> t = lam mf kindu (lam mf kindu (bound 0)) := sorry
-  lemma erase_cff_eq : erase t = erase cff -> t = lam mf kindu (lam mf kindu (bound 1)) := sorry
+  -- lemma erase_no_eqind : erase f ≠ J @τ t1 @τ t2 @0 t3 @0 t4 @ω t5 := sorry
+
+  -- lemma erase_free_invariant :
+  --   x ∉ (fv ∘ erase) ({_|-> x}t) ->
+  --   (y : Name) -> y ∉ fv t ->
+  --   erase ({_|-> x}t) = erase ({_|-> y}t)
+  -- := sorry
+
+  -- lemma erase_ctt_eq : erase t = erase ctt -> t = lam mf kindu (lam mf kindu (bound 0)) := sorry
+  -- lemma erase_cff_eq : erase t = erase cff -> t = lam mf kindu (lam mf kindu (bound 1)) := sorry
 
 end Cedille
