Cedille/Lemma/RedErasure.lean
@@ -1,94 +1,279 @@
 
+import Common
 import Cedille.Def
+import Cedille.Lemma.Basic
 import Cedille.Lemma.Refold
 import Cedille.Lemma.Erasure
+import Cedille.Lemma.Inversion
 import Cedille.Lemma.Red
 
 namespace Cedille
 
-  lemma red_erasure_step :
+  lemma erase_free_red :
+    ((x : Name) -> x ∉ fv t -> x ∉ (fv ∘ erase) ({_|-> x}t)) ->
+    (∃ x, {_|-> x}t -β>* {_|-> x}t') ->
+    (x : Name) -> x ∉ fv t' -> x ∉ (fv ∘ erase) ({_|-> x}t')
+  := sorry
+
+  -- lemma red_erasure_step_lam_mf :
+  --   erase t1 = lam mf kindu (erase t2) ->
+  --   t1 -β> z1 ->
+  --   ∃ z2, t2 -β>* z2 ∧ erase z1 = lam mf kindu (erase z2)
+  -- := sorry
+
+  -- lemma red_erasure_step_lam_mt {n} {t1 t2 z1 : Term n} {t2' : Term (n + 1)} :
+  --   erase t1 = lam mt (erase t2) (erase t2') ->
+  --   t1 -β> z1 ->
+  --   ∃ z2 z2', t2 -β>* z2 ∧ t2' -β>* z2' ∧ erase z1 = lam mt (erase z2) (erase z2')
+  -- := λ h step => @Nat.rec
+  --   (λ n =>
+  --     ∀ m (t1 t2 z1 : Term m) (t2' : Term (m + 1)),
+  --     size t1 ≤ n ->
+  --     erase t1 = lam mt (erase t2) (erase t2') ->
+  --     t1 -β> z1 ->
+  --     ∃ z2 z2', t2 -β>* z2 ∧ t2' -β>* z2' ∧ erase z1 = lam mt (erase z2) (erase z2'))
+  --   sorry
+  --   (by {
+  --     intros n ih m t1 t2 z1 t2' h e step
+  --     cases t1 <;> simp at * <;> simp
+  --     case const => cases step
+  --     case bind k u1 u2 => {
+  --       cases k <;> simp at *
+  --       case lam m =>
+  --       cases m <;> simp at *
+  --       case erased => {
+  --         generalize xdef : Name.fresh (fv u2) = x at *
+  --         cases step <;> simp at * <;> simp
+  --         case bind1 u1' step => {
+  --           exists t2; apply And.intro RedStar.refl _
+  --           exists t2'; apply And.intro RedStar.refl _
+  --           simp [*]
+  --         }
+  --         case bind2 u2' S step => {
+  --           have step : u2 -β> u2' := sorry
+  --           sorry
+  --         }
+  --       }
+  --       case type => {
+  --         sorry
+  --       }
+  --     }
+  --     case ctor => {
+  --       sorry
+  --     }
+  --   })
+  --   (size t1)
+  --   n
+  --   t1
+  --   t2
+  --   z1
+  --   t2'
+  --   (by simp)
+  --   h
+  --   step
+
+
+  lemma red_erasure_step2 :
+    Γ1 ⊢ t1 : A1 ->
+    Γ2 ⊢ t2 : A2 ->
     erase t1 = erase t2 ->
     t1 -β> z1 ->
     ∃ z2, t2 -β>* z2 ∧ erase z1 = erase z2
-  := λ h step => @Nat.subInduction
-    (λ n1 n2 =>
-      (t1 t2 z1 : _) ->
-      size t1 ≤ n1  ->
-      size t2 ≤ n2 ->
+  := λ j1 j2 h step => @Nat.rec
+    (λ n => 
+      ∀ Γ1 t1 A1 Γ2 t2 A2 z1,
+      size t2 ≤ n ->
+      Γ1 ⊢ t1 : A1 ->
+      Γ2 ⊢ t2 : A2 ->
       erase t1 = erase t2 ->
       t1 -β> z1 ->
       ∃ z2, t2 -β>* z2 ∧ erase z1 = erase z2)
+    sorry
     (by {
-      intros m t1 t2 z1 h1 h2 e step
-      have lem : size t1 = 0 := sorry
-      cases t1 <;> simp at lem <;> cases step
-    })
-    (by {
-      intros n t1 t2 z1 h1 h2 e step
-      sorry
-    })
-    (by {
-      intros n m ih t1 t2 z1 h1 h2 e step
-      cases t1 <;> cases t2 <;> simp at * <;> simp
-      case bound.bound _ => cases step
-      case bound.free _ => cases step
-      case bound.const _ => cases step
-      case bound.bind _ => cases step
-      case bound.ctor _ => cases step
-      case free.bound _ => cases step
-      case free.free _ => cases step
-      case free.const _ => cases step
-      case free.bind _ => cases step
-      case free.ctor _ => cases step
-      case const.bound _ => cases step
-      case const.free _ => cases step
-      case const.const _ => cases step
-      case const.bind _ => cases step
-      case const.ctor _ => cases step
-      case bind.bound _ q1 qstep k u1 u2 i => {
-        cases k
+      intros n ih Γ1 t1 A1 Γ2 t2 A2 z1 h j1 j2 e step
+      cases t2 <;> simp at * <;> simp
+      case bound i => apply ih Γ1 t1 A1 Γ2 (bound i) A2 z1 (by simp) j1 j2 e step
+      case free x => apply ih Γ1 t1 A1 Γ2 (free x) A2 z1 (by simp) j1 j2 e step
+      case const k => apply ih Γ1 t1 A1 Γ2 (const k) A2 z1 (by simp) j1 j2 e step
+      case bind k1 u1 u2 => {
+        cases k1
         case lam m => {
-          cases m <;> simp at * <;> simp [*]
+          cases m <;> simp at * <;> simp
+          case free => {
+            sorry
+            -- have lem := red_erasure_step_lam_mf e step
+            -- casesm* ∃ _, _, _ ∧ _; case _ w step2 e2 =>
+            -- exists lam mf u1 w; apply And.intro _ _
+            -- apply red_lam RedStar.refl step2
+            -- simp [*]
+          }
+          case type => {
+            sorry
+            -- have lem := red_erasure_step_lam_mt e step
+            -- casesm* ∃ _, _, _ ∧ _; case _ w1 w2 wstep1 wstep2 e2 =>
+            -- exists lam mt w1 w2; apply And.intro _ _
+            -- apply red_lam wstep1 wstep2
+            -- simp [*]
+          }
+          case erased => {
+            cases j2; case _ K B S g1 g2 g3 =>
+            have fresh := @Name.fresh_is_fresh (S ++ fv u2)
+            generalize xdef : Name.fresh (S ++ fv u2) = x at *
+            have xn1 := FvSet.not_mem_left fresh
+            have xn2 := FvSet.not_mem_right fresh
+            replace g3 := g3 x xn1
+            have g2r := erase_free_rename (g2 rfl)
+            have su2 : size ({_|-> x}u2) ≤ n := by {
+              have lem1 := Nat.le_of_succ_le_succ h
+              have lem2 := nat_add_le lem1
+              casesm* _ ∧ _; case _ l r =>
+              simp [*]
+            }
+            have e2 : erase t1 = erase ({_|-> x}u2) := by
+              rw [g2r x (Name.fresh (fv u2)) xn2 Name.fresh_is_fresh]; simp [*]
+            have lem := ih Γ1 t1 A1 (Γ2 ++ [x:u1]) ({_|-> x}u2) ({_|-> x}B) z1 su2 j1 g3 e2 step
+            casesm* ∃ _, _, _ ∧ _; case _ u2' ustep ue =>
+            have ustep2 := red_open_forced ustep
+            cases ustep2; case _ z zh =>
+            cases zh; case _ ze zn =>
+            subst ze
+            exists (lam m0 u1 z); apply And.intro _ _
+            apply red_lam RedStar.refl ustep; simp
+            have yfresh := @Name.fresh_is_fresh (fv z)
+            generalize ydef : Name.fresh (fv z) = y at *
+            have g2r2 := erase_free_rename (erase_free_red (g2 rfl) (Exists.intro x ustep))
+            have fv1 : fv z ⊆ fv u2 := fv_open_shrink zn (red_fv ustep)
+            have xn3 := contra (@subset_mem x (fv z) (fv u2) fv1) xn2
+            have e3 := g2r2 x y xn3 yfresh; simp at e3
+            rw [<-e3, ue]
+          }
         }
         case pi m => {
-
+          sorry
         }
         case inter => {
-
+          sorry
+        }
+      }
+      case ctor k u1 u2 u3 => {
+        cases k <;> simp at * <;> simp
+        case app => sorry
+        case pair => sorry
+        case fst => sorry
+        case snd => sorry
+        case eq => sorry
+        case refl => sorry
+        case eqind => sorry
+        case promote => sorry
+        case delta => sorry
+        case phi => {
+          cases j2; case _ A B g1 g2 g3 g4 g5 =>
+          cases g1; case _ A' g eq =>
+          have lem := ih Γ1 t1 A1 Γ2 u1 A' z1 sorry j1 g e step
+          casesm* ∃ _, _, _ ∧ _; case _ w step e =>
+          exists (phi w u2 u3); apply And.intro _ _
+          apply red_phi step RedStar.refl RedStar.refl
+          simp [*]
         }
       }
     })
-    (size t1)
     (size t2)
+    Γ1
     t1
+    A1
+    Γ2
     t2
+    A2
     z1
     (by simp)
-    (by simp)
+    j1
+    j2
     h
     step
 
+  -- lemma red_erasure_step {n} {t1 t2 z1 : Term n} :
+  --   erase t1 = erase t2 ->
+  --   t1 -β> z1 ->
+  --   ∃ z2, t2 -β>* z2 ∧ erase z1 = erase z2
+  -- := λ h step => @Nat.rec
+  --   (λ n => 
+  --     ∀ m (t1 t2 z1 : Term m),
+  --     size t1 ≤ n ->
+  --     erase t1 = erase t2 ->
+  --     t1 -β> z1 ->
+  --     ∃ z2, t2 -β>* z2 ∧ erase z1 = erase z2)
+  --   sorry
+  --   (by {
+  --     intros n ih m t1 t2 z1 h e step
+  --     cases t1
+  --     case bound => cases step
+  --     case free => cases step
+  --     case const => cases step
+  --     case bind k u1 u2 => {
+  --       cases k
+  --       case lam m => {
+  --         cases m; simp at *
+  --         case free => {
+  --           cases step <;> simp
+  --           case bind1 v1 step => {
+  --             exists t2; simp [*]
+  --             apply RedStar.refl
+  --           }
+  --           case bind2 v2 S step => {
+  --             have fresh := @Name.fresh_is_fresh S
+  --             generalize xdef : Name.fresh S = x at *
+  --             replace step := step x fresh
+  --             have lem := ih m ({_|-> x}u2) (t2) ({_|-> x}v2) sorry sorry step
+              
+  --           }
+  --         }
+  --         case type => {
 
+  --         }
+  --         case erased => {
+
+  --         }
+  --       }
+  --       case pi m => {
+
+  --       }
+  --       case inter => {
+
+  --       }
+  --     }
+  --     case ctor => {
+
+  --     }
+  --   })
+  --   (size t1)
+  --   n
+  --   t1
+  --   t2
+  --   z1
+  --   (by simp)
+  --   h
+  --   step
 
   lemma red_erasure :
     erase t1 = erase t2 ->
     t1 -β>* z1 ->
     ∃ z2, t2 -β>* z2 ∧ erase z1 = erase z2
-  := by {
-    intro h step
-    induction step generalizing t2
-    case refl t' => {
-      exists t2; simp [*]
-      apply RedStar.refl
-    }
-    case step u1 u2 u3 s1 _s2 e => {
-      have lem := red_erasure_step h s1
-      casesm* ∃ _, _, _ ∧ _; case _ w step e2 =>
-      have lem := @e w e2
-      casesm* ∃ _, _, _ ∧ _; case _ w' step' e3 =>
-      exists w'; simp [*]
-      apply RedStar.trans step step'
-    }
-  }
+  := by sorry
+  -- := by {
+  --   intro h step
+  --   induction step generalizing t2
+  --   case refl t' => {
+  --     exists t2; simp [*]
+  --     apply RedStar.refl
+  --   }
+  --   case step u1 u2 u3 s1 _s2 e => {
+  --     have lem := red_erasure_step h s1
+  --     casesm* ∃ _, _, _ ∧ _; case _ w step e2 =>
+  --     have lem := @e w e2
+  --     casesm* ∃ _, _, _ ∧ _; case _ w' step' e3 =>
+  --     exists w'; simp [*]
+  --     apply RedStar.trans step step'
+  --   }
+  -- }
 
 end Cedille
