Cedille/Lemma/Syntax.lean
@@ -1,0 +1,437 @@
+
+import Cedille.Def
+import Cedille.Lemma.Basic
+import Cedille.Lemma.Refold
+
+namespace Cedille
+
+  @[simp] lemma opn_head_const {n} : {_|-> x}(@const (n + 1) c) = @const n c := by congr
+  @[simp] lemma opn_head_free {n} : {_|-> y}(@free (n + 1) x) = free x := by congr
+  
+  @[simp] lemma opn_head_bound {n} {j : Fin n}
+    : {_|-> x}(@bound (n + 1) j) = if j == n then free x else bound j
+  := by {
+    unfold HasHOpen.hopn; unfold Syntax.instHasHOpenSyntax; simp
+    unfold Syntax.opn_head; unfold bound; simp
+  }
+
+  @[simp] lemma opn_head_bound2 {n}
+    : {_|-> x}(@bound (n + 1) ↑n) = free x
+  := by {
+    unfold HasHOpen.hopn; unfold Syntax.instHasHOpenSyntax; simp
+    unfold Syntax.opn_head; unfold bound; simp
+  }
+
+  @[simp] lemma opn_head_bound3 {n}
+    : {_|-> x}(@bound (n + 2) (↑n + 1)) = free x
+  := by {
+    unfold HasHOpen.hopn; unfold Syntax.instHasHOpenSyntax; simp
+    unfold Syntax.opn_head; unfold bound; simp
+    intro h
+    exfalso; apply h _
+    rw [Fin.val_add]; simp
+  }
+
+  @[simp] lemma opn_head_typeu : {_|-> x}typeu = @typeu n := by unfold typeu; simp
+  @[simp] lemma opn_head_kindu : {_|-> x}kindu = @kindu n := by unfold kindu; simp
+  @[simp] lemma opn_head_lam : {_|-> x}lam m t1 t2 = lam m ({_|-> x}t1) ({_|-> x}t2)
+    := by unfold lam; rw [Syntax.opn_head_bind]
+  @[simp] lemma opn_head_pi : {_|-> x}pi m t1 t2 = pi m ({_|-> x}t1) ({_|-> x}t2)
+    := by unfold pi; rw [Syntax.opn_head_bind]
+  @[simp] lemma opn_head_inter : {_|-> x}inter t1 t2 = inter ({_|-> x}t1) ({_|-> x}t2)
+    := by unfold inter; rw [Syntax.opn_head_bind]
+  @[simp] lemma opn_head_app : {_|-> x}app m t1 t2 = app m ({_|-> x}t1) ({_|-> x}t2)
+    := by unfold app; rw [Syntax.opn_head_ctor]; simp
+  @[simp] lemma opn_head_pair : {_|-> x}pair t1 t2 t3 = pair ({_|-> x}t1) ({_|-> x}t2) ({_|-> x}t3)
+    := by unfold pair; rw [Syntax.opn_head_ctor]
+  @[simp] lemma opn_head_fst : {_|-> x}fst t = fst ({_|-> x}t)
+    := by unfold fst; rw [Syntax.opn_head_ctor]; simp
+  @[simp] lemma opn_head_snd :{_|-> x}snd t = snd ({_|-> x}t) 
+    := by unfold snd; rw [Syntax.opn_head_ctor]; simp
+  @[simp] lemma opn_head_eq : {_|-> x}eq t1 t2 t3 = eq ({_|-> x}t1) ({_|-> x}t2) ({_|-> x}t3)
+    := by unfold eq; rw [Syntax.opn_head_ctor]
+  @[simp] lemma opn_head_refl : {_|-> x}refl t = refl ({_|-> x}t)
+    := by unfold refl; rw [Syntax.opn_head_ctor]; simp
+  @[simp] lemma opn_head_J {n} : {_|-> x}J = @J n
+    := by unfold J; rw [Syntax.opn_head_ctor]; simp
+  @[simp] lemma opn_head_promote : {_|-> x}promote t = promote ({_|-> x}t) 
+    := by unfold promote; rw [Syntax.opn_head_ctor]; simp
+  @[simp] lemma opn_head_delta : {_|-> x}delta t = delta ({_|-> x}t)
+    := by unfold delta; rw [Syntax.opn_head_ctor]; simp
+  @[simp] lemma opn_head_phi : {_|-> x}phi t1 t2 t3 = phi ({_|-> x}t1) ({_|-> x}t2) ({_|-> x}t3)
+    := by unfold phi; rw [Syntax.opn_head_ctor]
+
+  @[simp] lemma cls_head_const : {_<-| x}(@const n c) = const c := by congr
+  @[simp] lemma cls_head_bound : {_<-| x}(@bound n i) = @bound (n + 1) i := by congr
+
+  @[simp] lemma cls_head_free
+    : {_<-| v}(@free n x) = if x == v then bound n else free x
+  := by {
+    unfold HasHClose.hcls; unfold Syntax.instHasHCloseSyntax; simp
+    unfold Syntax.cls_head; unfold free; simp
+  }
+
+  @[simp] lemma cls_head_typeu : {_<-| x}@typeu n = typeu := by unfold typeu; simp
+  @[simp] lemma cls_head_kindu : {_<-| x}@kindu n = kindu := by unfold kindu; simp
+  @[simp] lemma cls_head_lam : {_<-| x}lam m t1 t2 = lam m ({_<-| x}t1) ({_<-| x}t2)
+    := by unfold lam; rw [Syntax.cls_head_bind]
+  @[simp] lemma cls_head_pi : {_<-| x}pi m t1 t2 = pi m ({_<-| x}t1) ({_<-| x}t2)
+    := by unfold pi; rw [Syntax.cls_head_bind]
+  @[simp] lemma cls_head_inter : {_<-| x}inter t1 t2 = inter ({_<-| x}t1) ({_<-| x}t2)
+    := by unfold inter; rw [Syntax.cls_head_bind]
+  @[simp] lemma cls_head_app : {_<-| x}app m t1 t2 = app m ({_<-| x}t1) ({_<-| x}t2)
+    := by unfold app; rw [Syntax.cls_head_ctor]; simp
+  @[simp] lemma cls_head_pair : {_<-| x}pair t1 t2 t3 = pair ({_<-| x}t1) ({_<-| x}t2) ({_<-| x}t3)
+    := by unfold pair; rw [Syntax.cls_head_ctor]
+  @[simp] lemma cls_head_fst : {_<-| x}fst t = fst ({_<-| x}t)
+    := by unfold fst; rw [Syntax.cls_head_ctor]; simp
+  @[simp] lemma cls_head_snd :{_<-| x}snd t = snd ({_<-| x}t) 
+    := by unfold snd; rw [Syntax.cls_head_ctor]; simp
+  @[simp] lemma cls_head_eq : {_<-| x}eq t1 t2 t3 = eq ({_<-| x}t1) ({_<-| x}t2) ({_<-| x}t3)
+    := by unfold eq; rw [Syntax.cls_head_ctor]
+  @[simp] lemma cls_head_refl : {_<-| x}refl t = refl ({_<-| x}t)
+    := by unfold refl; rw [Syntax.cls_head_ctor]; simp
+  @[simp] lemma cls_head_J {n} : {_<-| x}@J n = J
+    := by unfold J; rw [Syntax.cls_head_ctor]; simp
+  @[simp] lemma cls_head_promote : {_<-| x}promote t = promote ({_<-| x}t) 
+    := by unfold promote; rw [Syntax.cls_head_ctor]; simp
+  @[simp] lemma cls_head_delta : {_<-| x}delta t = delta ({_<-| x}t)
+    := by unfold delta; rw [Syntax.cls_head_ctor]; simp
+  @[simp] lemma cls_head_phi : {_<-| x}phi t1 t2 t3 = phi ({_<-| x}t1) ({_<-| x}t2) ({_<-| x}t3)
+    := by unfold phi; rw [Syntax.cls_head_ctor]
+
+  @[simp] lemma hsubst_const {v : Term n} : [_:= v](@const (n + 1) c) = const c := by congr
+  @[simp] lemma hsubst_free {v : Term n} : [_:= v](@free (n + 1) x) = free x
+  := by unfold free; rw [Syntax.hsubst_free]
+
+  @[simp] lemma hsubst_typeu {v : Term n} : [_:= v]@typeu (n + 1) = typeu
+    := by unfold typeu; rw [Syntax.hsubst_const]
+  @[simp] lemma hsubst_kindu {v : Term n} : [_:= v]@kindu (n + 1) = kindu
+    := by unfold kindu; rw [Syntax.hsubst_const]
+  @[simp] lemma hsubst_lam {v : Term n}
+    : [_:= v]lam m t1 t2 = lam m ([_:= v]t1) ([_:= (Syntax.weaken v 1)]t2)
+    := by unfold lam; rw [Syntax.hsubst_bind]
+  @[simp] lemma hsubst_pi {v : Term n}
+    : [_:= v]pi m t1 t2 = pi m ([_:= v]t1) ([_:= (Syntax.weaken v 1)]t2)
+    := by unfold pi; rw [Syntax.hsubst_bind]
+  @[simp] lemma hsubst_inter {v : Term n}
+    : [_:= v]inter t1 t2 = inter ([_:= v]t1) ([_:= (Syntax.weaken v 1)]t2)
+    := by unfold inter; rw [Syntax.hsubst_bind]
+  @[simp] lemma hsubst_app {v : Term n} : [_:= v]app m t1 t2 = app m ([_:= v]t1) ([_:= v]t2)
+    := by unfold app; rw [Syntax.hsubst_ctor]; simp
+  @[simp] lemma hsubst_pair {v : Term n}
+    : [_:= v]pair t1 t2 t3 = pair ([_:= v]t1) ([_:= v]t2) ([_:= v]t3)
+    := by unfold pair; rw [Syntax.hsubst_ctor]
+  @[simp] lemma hsubst_fst {v : Term n} : [_:= v]fst t = fst ([_:= v]t)
+    := by unfold fst; rw [Syntax.hsubst_ctor]; simp
+  @[simp] lemma hsubst_snd {v : Term n} : [_:= v]snd t = snd ([_:= v]t) 
+    := by unfold snd; rw [Syntax.hsubst_ctor]; simp
+  @[simp] lemma hsubst_eq {v : Term n} : [_:= v]eq t1 t2 t3 = eq ([_:= v]t1) ([_:= v]t2) ([_:= v]t3)
+    := by unfold eq; rw [Syntax.hsubst_ctor]
+  @[simp] lemma hsubst_refl {v : Term n} : [_:= v]refl t = refl ([_:= v]t)
+    := by unfold refl; rw [Syntax.hsubst_ctor]; simp
+  @[simp] lemma hsubst_J {n} {v : Term n} : [_:= v]@J (n + 1) = J
+    := by unfold J; rw [Syntax.hsubst_ctor]; simp
+  @[simp] lemma hsubst_promote {v : Term n} : [_:= v]promote t = promote ([_:= v]t) 
+    := by unfold promote; rw [Syntax.hsubst_ctor]; simp
+  @[simp] lemma hsubst_delta {v : Term n} : [_:= v]delta t = delta ([_:= v]t)
+    := by unfold delta; rw [Syntax.hsubst_ctor]; simp
+  @[simp] lemma hsubst_phi {v : Term n} : [_:= v]phi t1 t2 t3 = phi ([_:= v]t1) ([_:= v]t2) ([_:= v]t3)
+    := by unfold phi; rw [Syntax.hsubst_ctor]
+
+  lemma close_open_cancel {n} {t : Term (n + 1)} : x ∉ fv t -> {_<-| x}{_|-> x}t = t
+    := λ h => @Nat.rec
+      (λ n =>
+        ∀ x m (t : Term (m + 1)),
+        size t ≤ n ->
+        x ∉ fv t ->
+        {_<-| x}{_|-> x}t = t)
+      (by {
+        intro x m t e h
+        cases t <;> simp at *
+        case bound i => {
+          unfold HasHOpen.hopn; unfold Syntax.instHasHOpenSyntax
+          unfold Syntax.opn_head; unfold bound; simp
+          split
+          case _ h => {
+            simp; cases i; case _ iv il =>
+            simp at *; subst h
+            rw [fin_cast il]; exact iv
+          }
+          case _ h => simp; rw [<-fin_cast2]
+        }
+        case free y => {
+          intro h2
+          have h3 : x = y := by rw [h2]
+          exfalso; apply h h3
+        }
+      })
+      (by {
+        intro m ih x k t e h
+        cases t <;> simp at *
+        case bound i => {
+          unfold HasHOpen.hopn; unfold Syntax.instHasHOpenSyntax
+          unfold Syntax.opn_head; unfold bound; simp
+          split
+          case _ h => {
+            simp; cases i; case _ iv il =>
+            simp at *; subst h
+            rw [fin_cast il]; exact iv
+          }
+          case _ h => simp; rw [<-fin_cast2]
+        }
+        case free y => {
+          intro h2
+          have h3 : x = y := by rw [h2]
+          exfalso; apply h h3
+        }
+        case bind b u1 u2 => {
+          have e1 : size u1 ≤ m := by linarith
+          have e2 : size u2 ≤ m := by linarith
+          have h := demorgan h
+          cases h; case _ l r =>
+          rw [ih x k u1 e1 l, ih x (k + 1) u2 e2 r]
+          simp
+        }
+        case ctor c u1 u2 u3 => {
+          have e1 : size u1 ≤ m := by linarith
+          have e2 : size u2 ≤ m := by linarith
+          have e3 : size u3 ≤ m := by linarith
+          have h := demorgan h
+          cases h; case _ l r =>
+          have h := demorgan r
+          cases h; case _ r1 r2 =>
+          rw [ih x k u1 e1 l, ih x k u2 e2 r1, ih x k u3 e3 r2]
+          simp
+        }
+      })
+      (size t)
+      x
+      n
+      t
+      (by simp)
+      h
+
+  lemma open_to_close {n} {t1 : Term (n + 1)} {t2 : Term n}
+    : x ∉ fv t1 -> {_|-> x}t1 = t2 -> t1 = {_<-| x}t2
+  := by {
+    intro xn h
+    have h2 : {_<-| x}{_|-> x}t1 = {_<-| x}t2 := by congr
+    rw [close_open_cancel xn] at h2
+    exact h2
+  }
+
+  lemma var_not_in_close {n} {t : Term n} : x ∉ fv ({_<-| x}t) := by {
+    intro h
+    induction t <;> simp at *
+    case free m y => {
+      split at h
+      case _ => simp at h
+      case _ h2 => {
+        simp at h
+        subst h; simp at h2
+      }
+    }
+    case bind m b u1 u2 ih1 ih2 => {
+      cases h
+      case inl h => apply ih1 h
+      case inr h => apply ih2 h
+    }
+    case ctor m c u1 u2 u3 ih1 ih2 ih3 => {
+      cases h
+      case _ h => apply ih1 h
+      case _ h => {
+        cases h
+        case _ h => apply ih2 h
+        case _ h => apply ih3 h
+      }
+    }
+  }
+
+  lemma fv_open_shrink {n} {t1 t2 : Term (n + 1)}
+    : x ∉ fv t1 -> fv ({_|-> x}t1) ⊆ fv ({_|-> x}t2) -> fv t1 ⊆ fv t2
+  := λ h1 h2 => @Nat.rec
+    (λ n =>
+      ∀ m1 m2 (t1 : Term (m1 + 1)) (t2 : Term (m2 + 1)),
+      size t1 ≤ n ->
+      x ∉ fv t1 ->
+      fv ({_|-> x}t1) ⊆ fv ({_|-> x}t2) ->
+      fv t1 ⊆ fv t2)
+    (by {
+      intro m1 m2 t1 t2 e h1 h2
+      cases t1 <;> simp at *
+      case free y _ => {
+        cases h2 <;> simp [*]
+        case _ h =>
+        have h : x = y := by rw [h]
+        exfalso; apply h1 h
+      }
+    })
+    (by {
+      intro n ih m1 m2 t1 t2 e h1 h2
+      cases t1
+      case bound i => apply ih m1 m2 (bound i) t2 (by simp) h1 h2
+      case free x => apply ih m1 m2 (free x) t2 (by simp) h1 h2
+      case const k => apply ih m1 m2 (const k) t2 (by simp) h1 h2
+      case bind b u1 u2 => {
+        simp at *
+        have e1 : size u1 ≤ n := by linarith
+        have e2 : size u2 ≤ n := by linarith
+        cases h2; case _ h21 h22 =>
+        cases (demorgan h1); case _ h11 h12 =>
+        apply And.intro _ _
+        apply ih _ _ _ _ e1 h11 h21
+        apply ih _ _ u2 t2 e2 h12 h22
+      }
+      case ctor c u1 u2 u3 => {
+        simp at *
+        have e1 : size u1 ≤ n := by linarith
+        have e2 : size u2 ≤ n := by linarith
+        have e3 : size u3 ≤ n := by linarith
+        have h1 := demorgan h1
+        cases h1; case _ h11 h1 =>
+        cases (demorgan h1); case _ h12 h13 =>
+        cases h2; case _ h21 h2 =>
+        cases h2; case _ h22 h23 =>
+        apply And.intro _ _
+        apply ih _ _ _ _ e1 h11 h21
+        apply And.intro _ _
+        apply ih _ _ _ _ e2 h12 h22
+        apply ih _ _ _ _ e3 h13 h23
+      }
+    })
+    (size t1)
+    n
+    n
+    t1
+    t2
+    (by simp)
+    h1
+    h2
+
+  @[simp↓ high] lemma rename_bound {i : Fin n} : {_|-> x}{_<-| y}(@bound n i) = bound i
+  := by unfold bound; rw [Syntax.rename_bound]
+
+  lemma rename_free_neq : z ≠ y -> {_|-> x}{_<-| y}(@free n z) = free z
+  := by intro h; unfold free; rw [Syntax.rename_free_neq h]
+
+  lemma rename_free_eq : {_|-> x}{_<-| y}(@free n y) = free x
+  := by unfold free; rw [Syntax.rename_free_eq]
+
+  @[simp] lemma rename_subst_commute (x y) {n} {t1 : Term n} {t2 : Term (n + 1)} :
+    {_|-> y}{_<-| x}[_:= t1]t2 = [_:= {_|-> y}{_<-| x}t1]({_|-> y}{_<-| x}t2)
+  := @Nat.rec
+    (λ m => ∀ n (t1 : Term n) (t2 : Term (n + 1)),
+      size t2 ≤ m ->
+      {_|-> y}{_<-| x}[_:= t1]t2 = [_:= {_|-> y}{_<-| x}t1]({_|-> y}{_<-| x}t2))
+    (by {
+      intros m t1 t2 h
+      cases t2 <;> simp at h
+      case bound i => {
+        unfold HasHSubst.hsubst; unfold Syntax.instHasHSubstSyntax; simp
+        unfold Syntax.hsubst; unfold bound; simp
+        split; simp
+        rw [rename_bound]
+      }
+      case free z => simp; split <;> simp
+      case const => simp
+    })
+    (by {
+      intro m ih n t1 t2 h
+      cases t2 <;> simp at h
+      case bound => apply ih n t1 (bound _) (by simp)
+      case free => apply ih n t1 (free _) (by simp)
+      case const => apply ih n t1 (const _) (by simp)
+      case bind b u1 u2 => {
+        have s1 : size u1 ≤ m := by linarith
+        have s2 : size u2 ≤ m := by linarith
+        simp; apply And.intro _ _
+        apply ih n t1 u1 s1
+        have lem := ih (n + 1) (Syntax.weaken t1 1) u2 s2
+        simp at lem
+        rw [lem]
+      }
+      case ctor c u1 u2 u3 => {
+        have s1 : size u1 ≤ m := by linarith
+        have s2 : size u2 ≤ m := by linarith
+        have s3 : size u3 ≤ m := by linarith
+        simp; apply And.intro _ _
+        apply ih n t1 u1 s1
+        apply And.intro _ _
+        apply ih n t1 u2 s2
+        apply ih n t1 u3 s3
+      }
+    })
+    (size t2)
+    n
+    t1
+    t2
+    (by simp)
+
+  lemma rename_open_commute {t : Term (n + 1)} : z ≠ x ->
+    {_|-> z}{_|-> y}{_<-| x}t = {_|-> y}{_<-| x}{_|-> z}t
+  := λ h1 => @Nat.rec
+    (λ m => ∀ n (t : Term (n + 1)),
+      size t ≤ m ->
+      {_|-> z}{_|-> y}{_<-| x}t = {_|-> y}{_<-| x}{_|-> z}t)
+    (by {
+      intro n t s
+      cases t <;> simp at s
+      case bound i => {
+        simp
+        generalize hdef : {_|-> z}bound i = h
+        unfold HasHOpen.hopn at hdef; unfold Syntax.instHasHOpenSyntax at hdef
+        simp at hdef; unfold Syntax.opn_head at hdef; unfold bound at hdef; simp at hdef
+        split at hdef
+        case _ h => {
+          rw [<-hdef]; simp
+          rw [Name.beq_of_not_eq h1]; simp
+        }
+        case _ h => rw [<-hdef]; simp
+      }
+      case free w => {
+        generalize hdef : {_|-> z}Syntax.free w = h
+        simp at hdef; rw [<-hdef]; unfold free
+        cases Name.decEq w x
+        case isFalse h => {
+          rw [Syntax.rename_free_neq h, Syntax.rename_free_neq h]
+          simp
+        }
+        case isTrue h => {
+          subst h
+          rw [Syntax.rename_free_eq, Syntax.rename_free_eq]
+          simp
+        }
+      }
+      case const => simp
+    })
+    (by {
+      intro m ih n t s
+      cases t
+      case bound => apply ih n (bound _) (by simp)
+      case free => apply ih n (free _) (by simp)
+      case const => apply ih n (const _) (by simp)
+      case bind b u1 u2 => {
+        simp at *
+        have s1 : size u1 ≤ m := by linarith
+        have s2 : size u2 ≤ m := by linarith
+        apply And.intro _ _
+        apply ih n u1 s1; apply ih (n + 1) u2 s2
+      }
+      case ctor c u1 u2 u3 => {
+        simp at *
+        have s1 : size u1 ≤ m := by linarith
+        have s2 : size u2 ≤ m := by linarith
+        have s3 : size u3 ≤ m := by linarith
+        apply And.intro _ _
+        apply ih n u1 s1
+        apply And.intro _ _
+        apply ih n u2 s2; apply ih n u3 s3
+      }
+    })
+    (size t)
+    n
+    t
+    (by simp)
+
+end Cedille
