Main.lean
@@ -1,0 +1,6 @@
+
+import Common
+import SystemFOmega
+import Cedille
+
+def main := IO.println "Hello, World!"
